Adjust semantics for binaries

src/StrictEqualities.v
@@ -7,72 +7,32 @@ Import ListNotations.
 Fixpoint Exp_eqb_strict (e1 e2 : Exp) : bool :=
   match e1, e2 with
   | VVal a, VVal a' => Val_eqb_strict a a'
-  | EExp (EValues l), EExp (EValues l') => 
-      (fix blist l l' := match l, l' with
-        | [], [] => true
-        | x::xs, x'::xs' => andb (Exp_eqb_strict x x') 
-                                 (blist xs xs')
-        | _, _ => false
-        end) l l'
-  | EExp (EFun vl e), EExp (EFun vl' e') => Nat.eqb vl vl' && Exp_eqb_strict e e'
-  | EExp (ECons hd tl), EExp (ECons hd' tl') => Exp_eqb_strict hd hd' && Exp_eqb_strict tl tl'
-  | EExp (ETuple l), EExp (ETuple l') => 
-      (fix blist l l' := match l, l' with
-        | [], [] => true
-        | x::xs, x'::xs' => andb (Exp_eqb_strict x x') (blist xs xs')
-        | _, _ => false
-        end) l l'
-  | EExp (ECall m f l), EExp (ECall m' f' l') => Exp_eqb_strict f f' && Exp_eqb_strict m m' && 
-      (fix blist l l' := match l, l' with
-        | [], [] => true
-        | x::xs, x'::xs' => andb (Exp_eqb_strict x x') (blist xs xs')
-        | _, _ => false
-        end) l l'
-  | EExp (EPrimOp f l), EExp (EPrimOp f' l') => String.eqb f f' && 
-      (fix blist l l' := match l, l' with
-        | [], [] => true
-        | x::xs, x'::xs' => andb (Exp_eqb_strict x x') (blist xs xs')
-        | _, _ => false
-        end) l l'
-  | EExp (EApp exp l), EExp (EApp exp' l') => Exp_eqb_strict exp exp' && 
-      (fix blist l l' := match l, l' with
-        | [], [] => true
-        | x::xs, x'::xs' => andb (Exp_eqb_strict x x') (blist xs xs')
-        | _, _ => false
-        end) l l'
-  | EExp (ECase e l), EExp (ECase e' l') => Exp_eqb_strict e e' 
-      && Nat.eqb (length l) (length l') 
-      && (fix blist l l' := match l, l' with
-        | [], [] => true
-        | (pl,y,z)::xs, (pl',y',z')::xs' => andb (
-          (fix blist l l' := match l, l' with
-          | [], [] => true
-          | x::xs, x'::xs' => andb (Pat_eqb x x') (blist xs xs')
-          | _, _ => false
-          end) pl pl') 
-          (andb (Exp_eqb_strict y y') (andb (Exp_eqb_strict z z') (blist xs xs')))
-                                           | _, _ => false
-                                           end) l l' 
-  | EExp (ELet l e1 e2), EExp (ELet l' e1' e2') => 
+  | EExp e1, EExp e2 => NonVal_eqb_strict e1 e2
+  | _, _ => false
+  end
+with NonVal_eqb_strict (e1 e2 : NonVal) : bool :=
+  match e1, e2 with
+  | EValues l, EValues l' => list_eqb Exp_eqb_strict l l'
+  | EFun vl e, EFun vl' e' => Nat.eqb vl vl' && Exp_eqb_strict e e'
+  | ECons hd tl, ECons hd' tl' => Exp_eqb_strict hd hd' && Exp_eqb_strict tl tl'
+  | ETuple l, ETuple l' => list_eqb Exp_eqb_strict l l'
+  | ECall m f l, ECall m' f' l' => Exp_eqb_strict f f' && Exp_eqb_strict m m' &&
+      list_eqb Exp_eqb_strict l l'
+  | EPrimOp f l, EPrimOp f' l' => String.eqb f f' && list_eqb Exp_eqb_strict l l'
+  | EApp exp l, EApp exp' l' => Exp_eqb_strict exp exp' && list_eqb Exp_eqb_strict l l'
+  | ECase e l, ECase e' l' => Exp_eqb_strict e e' 
+      && Nat.eqb (length l) (length l')
+      && list_eqb (prod_eqb (prod_eqb (list_eqb Pat_eqb_strict) Exp_eqb_strict) Exp_eqb_strict) l l'
+  | ELet l e1 e2, ELet l' e1' e2' => 
       Nat.eqb l l' && Exp_eqb_strict e1 e1' && Exp_eqb_strict e2 e2'
-  | EExp (ESeq e1 e2), EExp (ESeq e1' e2') => andb (Exp_eqb_strict e1 e1') (Exp_eqb_strict e2 e2')
-  | EExp (ELetRec l e), EExp (ELetRec l' e') => 
-      (fix blist l l' := match l, l' with
-        | [], [] => true
-        | (x,y)::xs, (x',y')::xs' => 
-        andb (Nat.eqb x x') (andb (Exp_eqb_strict y y') (blist xs xs'))
-        | _, _ => false
-        end) l l' && Exp_eqb_strict e e'
-  | EExp (EMap l), EExp (EMap l') => 
-      (fix blist l l' := match l, l' with
-        | [], [] => true
-        | (x,y)::xs, (x',y')::xs' => 
-        andb (Exp_eqb_strict x x') (andb (Exp_eqb_strict y y') (blist xs xs'))
-        | _, _ => false
-        end) l l'
-  | EExp (ETry e1 vl1 e2 vl2 e3), EExp (ETry e1' vl1' e2' vl2' e3') => 
+  | ESeq e1 e2, ESeq e1' e2' => andb (Exp_eqb_strict e1 e1') (Exp_eqb_strict e2 e2')
+  | ELetRec l e, ELetRec l' e' => list_eqb (prod_eqb Nat.eqb Exp_eqb_strict) l l' && Exp_eqb_strict e e'
+  | EMap l, EMap l' => list_eqb (prod_eqb Exp_eqb_strict Exp_eqb_strict) l l'
+  | ETry e1 vl1 e2 vl2 e3, ETry e1' vl1' e2' vl2' e3' => 
       Nat.eqb vl1 vl1' && Nat.eqb vl2 vl2' &&
       Exp_eqb_strict e1 e1' && Exp_eqb_strict e2 e2' && Exp_eqb_strict e3 e3'
+  | EBin l, EBin l'     => list_eqb Exp_eqb_strict l l'
+  | ESeg seg, ESeg seg' => Segment_eqb Exp_eqb_strict Exp_eqb_strict seg seg'
   | _, _ => false
   end
 with Val_eqb_strict (v1 v2 : Val) : bool :=
@@ -81,444 +41,342 @@ with Val_eqb_strict (v1 v2 : Val) : bool :=
   | VLit l, VLit l' => Lit_beq l l'
   | VPid p, VPid p' => Nat.eqb p p'
   | VCons hd tl, VCons hd' tl' => Val_eqb_strict hd hd' && Val_eqb_strict tl tl'
-  | VTuple l, VTuple l' => 
-      (fix blist l l' := match l, l' with
-        | [], [] => true
-        | x::xs, x'::xs' => andb (Val_eqb_strict x x') (blist xs xs')
-        | _, _ => false
-        end) l l'
-  | VMap l, VMap l' => 
-      (fix blist l l' := match l, l' with
-        | [], [] => true
-        | (x,y)::xs, (x',y')::xs' => 
-        andb (Val_eqb_strict x x') (andb (Val_eqb_strict y y') (blist xs xs'))
-        | _, _ => false
-        end) l l'
+  | VTuple l, VTuple l' => list_eqb Val_eqb_strict l l'
+  | VMap l, VMap l' => list_eqb (prod_eqb Val_eqb_strict Val_eqb_strict) l l'
   | VVar v, VVar v' => Nat.eqb v v'
   | VFunId v, VFunId v' => funid_eqb v v'
   | VClos ext id vc e, VClos ext' id' vc' e' => 
       Nat.eqb id id' && Nat.eqb vc vc' && Exp_eqb_strict e e' &&
-      (fix blist l l' := match l, l' with
-        | [], [] => true
-        | (n1,n2,e)::xs, (n1',n2',e')::xs' => 
-        andb (Exp_eqb_strict e e') (andb (Nat.eqb n1 n1') (andb (Nat.eqb n2 n2') (blist xs xs')))
-        | _, _ => false
-        end) ext ext'
+      list_eqb (prod_eqb (prod_eqb Nat.eqb Nat.eqb) Exp_eqb_strict) ext ext'
+  | VBitstring bits, VBitstring bits' => if bvn_eq_dec bits bits' then true else false
   | _, _ => false
-  end.
+  end
+with Pat_eqb_strict (p1 p2 : Pat) : bool :=
+match p1, p2 with
+| PVar, PVar => true
+| PLit l, PLit l' => Lit_beq l l'
+| PCons hd tl, PCons hd' tl' => Pat_eqb_strict hd hd' && Pat_eqb_strict tl tl'
+| PTuple l, PTuple l' => list_eqb Pat_eqb_strict l l'
+| PMap l, PMap l' => list_eqb (prod_eqb Pat_eqb_strict Pat_eqb_strict) l l'
+| PNil, PNil => true
+| PBin segs, PBin segs' => list_eqb (Segment_eqb Pat_eqb_strict Val_eqb_strict) segs segs'
+| _, _ => false
+end.
 
-Lemma Pat_eqb_refl: forall p, Pat_eqb p p = true.
+Theorem Private_eqb_strict_refl :
+     (forall e, Exp_eqb_strict e e = true)
+  /\ (forall e, NonVal_eqb_strict e e = true)
+  /\ (forall v, Val_eqb_strict v v = true)
+  /\ (forall p, Pat_eqb_strict p p = true).
 Proof.
-  induction p using Pat_ind2 with
-  (Q := Forall (fun p => Pat_eqb p p = true))
-  (R := Forall (PBoth (fun p => Pat_eqb p p = true))); simpl; auto.
-  * apply Lit_eqb_refl.
-  * now rewrite IHp1, IHp2.
-  * induction IHp; auto. now rewrite H, IHIHp.
-  * induction IHp; auto. destruct x, H. simpl in *. now rewrite H, H0, IHIHp.
-Qed.
-
-Lemma Pat_eqb_eq: forall p1 p2, Pat_eqb p1 p2 = true <-> p1 = p2.
-Proof.
-  intros. split.
-  * revert p2.
-    induction p1 using Pat_ind2 with
-    (Q := Forall (fun p => forall p2, Pat_eqb p p2 = true -> p = p2))
-    (R := Forall (PBoth (fun p => forall p2, Pat_eqb p p2 = true -> p = p2))); auto; intros.
-    + simpl in H. destruct p2; try discriminate. reflexivity.
-    + simpl in H. destruct p2; try discriminate. apply Lit_eqb_eq in H. subst. reflexivity.
-    + simpl in H. destruct p2; try discriminate. reflexivity.
-    + simpl in H. destruct p2; try discriminate.
-      apply andb_prop in H. destruct H.
-      apply IHp1_1 in H. apply IHp1_2 in H0. subst. reflexivity.
-    + simpl in H. destruct p2; try discriminate.
-      revert H IHp1. revert l0.
-      induction l; intros.
-      - destruct l0. reflexivity. discriminate.
-      - destruct l0. discriminate.
-        apply andb_prop in H. destruct H.
-        inv IHp1. apply H3 in H. subst a.
-        specialize (IHl l0 H0 H4). inv IHl. reflexivity.
-    + simpl in H. destruct p2; try discriminate.
-      revert H IHp1. revert l0.
-      induction l; intros.
-      - destruct l0. reflexivity. discriminate.
-      - destruct a. destruct l0. discriminate.
-        destruct p1. apply andb_prop in H. destruct H. apply andb_prop in H. destruct H.
-        inv IHp1. inv H4. apply H2 in H. apply H3 in H1. simpl in H, H1. subst.
-        specialize (IHl l0 H0 H5). inv IHl. reflexivity.
-  * intros. subst. apply Pat_eqb_refl.
-Qed.
-
-Lemma Exp_eqb_strict_refl: forall e, Exp_eqb_strict e e = true.
-Proof.
-  induction e using Exp_ind2 with
-    (PV := fun v => Val_eqb_strict v v = true)
-    (PE := fun e => Exp_eqb_strict e e = true)
-    (Q  := Forall (fun e => Exp_eqb_strict e e = true))
+  apply Exp_ind with
+    (Q := Forall (fun v => Exp_eqb_strict v v = true))
     (QV := Forall (fun v => Val_eqb_strict v v = true))
     (R  := Forall (PBoth (fun e => Exp_eqb_strict e e = true)))
     (RV := Forall (PBoth (fun v => Val_eqb_strict v v = true)))
-    (VV := Forall (fun e => Exp_eqb_strict e.2 e.2 = true))
-    (W  := Forall (fun '(e1, e2, e3) => Exp_eqb_strict e3 e3 = true 
-                    /\ Exp_eqb_strict e2 e2 = true
-                    /\ Forall (fun p => Pat_eqb p p = true) e1))
-    (Z  := Forall (fun e => Exp_eqb_strict e.2 e.2 = true)); simpl; auto.
+    (VV := Forall (fun '(_,_,e) => Exp_eqb_strict e e = true))
+    (W  := Forall (fun '(lp,e1,e2) => Forall (fun p => Pat_eqb_strict p p = true) lp
+                    /\ Exp_eqb_strict e1 e1 = true /\ Exp_eqb_strict e2 e2 = true))
+    (Z  := Forall (fun '(_,e) => Exp_eqb_strict e e = true))
+    (PQ := Forall (fun p => Pat_eqb_strict p p = true))
+    (PR := Forall (PBoth (fun p => Pat_eqb_strict p p = true)))
+    (PT := Forall (fun seg : Segment Pat Val => Pat_eqb_strict (Syntax.val seg) (Syntax.val seg) = true
+                    /\ Val_eqb_strict (Syntax.size seg) (Syntax.size seg) = true))
+  ; simpl; auto; intros.
+  (* Val *)
   * apply Lit_eqb_refl.
   * apply Nat.eqb_refl.
-  * rewrite IHe, IHe0. reflexivity.
-  * induction IHe; auto. rewrite H, IHIHe. reflexivity.
-  * induction IHe; auto. destruct x, H. simpl in *. rewrite H, H0, IHIHe. reflexivity.
+  * rewrite H, H0. reflexivity.
+  * induction H; auto. simpl. rewrite H, IHForall. reflexivity.
+  * induction H; auto. destruct x, H. simpl in *. simpl. rewrite H, H1, IHForall. reflexivity.
   * apply Nat.eqb_refl.
-  * destruct n. simpl. do 2 rewrite Nat.eqb_refl. reflexivity.
-  * rewrite IHe0, Nat.eqb_refl, Nat.eqb_refl. simpl.
-    clear -IHe. induction IHe; auto.
-    destruct x, p. simpl in H. rewrite IHIHe, H, Nat.eqb_refl, Nat.eqb_refl. reflexivity.
-  * now rewrite IHe, Nat.eqb_refl.
-  * induction IHe; auto. now rewrite H, IHIHe.
-  * now rewrite IHe1, IHe2.
-  * induction IHe; auto. now rewrite H, IHIHe.
-  * induction IHe; auto. destruct x, H. simpl in *. now rewrite H, H0, IHIHe.
-  * rewrite IHe1, IHe2. simpl.
-    clear -IHe3. induction IHe3; auto. now rewrite H, IHIHe3.
-  * rewrite String.eqb_refl. simpl. induction IHe; auto.
-    now rewrite H, IHIHe.
-  * rewrite IHe. simpl.
-    clear -IHe0. induction IHe0; auto. now rewrite H, IHIHe0.
-  * rewrite IHe, Nat.eqb_refl. simpl. induction IHe0; auto.
-    destruct x, p, H, H0. simpl in *. rewrite H, H0. simpl. rewrite IHIHe0.
-    clear -H1. induction H1; auto. rewrite H. simpl. rewrite IHForall. reflexivity.
-  * now rewrite IHe1, IHe2, Nat.eqb_refl.
-  * now rewrite IHe1, IHe2.
-  * rewrite IHe. induction IHe0; auto. destruct x. simpl in H.
-    rewrite Nat.eqb_refl. simpl in *. rewrite H. simpl. rewrite IHIHe0. reflexivity.
-  * now rewrite Nat.eqb_refl, Nat.eqb_refl, IHe1, IHe2, IHe3.
-  * constructor; auto.
-    split. auto. split. auto.
-    induction l; constructor. apply Pat_eqb_refl. apply IHl.
-Qed.
-
-Lemma Val_eqb_strict_refl: forall v, Val_eqb_strict v v = true.
-Proof.
-  induction v using Val_ind2 with
-    (P  := fun v => Exp_eqb_strict v v = true)
-    (PE := fun e => Exp_eqb_strict e e = true)
-    (Q  := Forall (fun e => Exp_eqb_strict e e = true))
-    (QV := Forall (fun v => Val_eqb_strict v v = true))
-    (R  := Forall (PBoth (fun e => Exp_eqb_strict e e = true)))
-    (RV := Forall (PBoth (fun v => Val_eqb_strict v v = true)))
-    (VV := Forall (fun e => Exp_eqb_strict e.2 e.2 = true))
-    (W  := Forall (fun '(e1, e2, e3) => Exp_eqb_strict e3 e3 = true 
-                    /\ Exp_eqb_strict e2 e2 = true
-                    /\ Forall (fun p => Pat_eqb p p = true) e1))
-    (Z  := Forall (fun e => Exp_eqb_strict e.2 e.2 = true)); simpl; auto.
+  * destruct n. simpl. now rewrite !Nat.eqb_refl.
+  * rewrite H0, Nat.eqb_refl, Nat.eqb_refl. simpl.
+    clear -H. induction H; auto.
+    destruct x, p. simpl in H. simpl. rewrite IHForall, H, Nat.eqb_refl, Nat.eqb_refl. reflexivity.
+  * destruct (bvn_eq_dec b b); [reflexivity | contradiction].
+  (* NonVal *)
+  * rewrite H, Nat.eqb_refl. reflexivity.
+  * induction H; auto. simpl. rewrite H, IHForall. reflexivity.
+  * rewrite H, H0. reflexivity.
+  * induction H; auto. simpl. rewrite H, IHForall. reflexivity.
+  * induction H; auto. destruct x, H. simpl in *. rewrite H, H1, IHForall. reflexivity.
+  * rewrite H, H0. simpl.
+    clear -H1. induction H1; auto. simpl. rewrite H, IHForall. reflexivity.
+  * rewrite String.eqb_refl. simpl. induction H; auto. simpl. rewrite H, IHForall. reflexivity.
+  * rewrite H. simpl.
+    clear -H0. induction H0; auto. simpl. rewrite H, IHForall. reflexivity.
+  * rewrite H, Nat.eqb_refl. simpl. induction H0; auto.
+    destruct x as [[lp e1] e2]. destruct H0 as [Hlp [He1 He2]].
+    assert (Hlpres : list_eqb Pat_eqb_strict lp lp = true).
+    { clear -Hlp. induction Hlp; auto. simpl. rewrite H, IHHlp. reflexivity. }
+    simpl. rewrite Hlpres, He1, He2, IHForall. reflexivity.
+  * rewrite H, H0, Nat.eqb_refl. reflexivity.
+  * rewrite H, H0. reflexivity.
+  * assert (Hlres : list_eqb (prod_eqb Nat.eqb Exp_eqb_strict) l l = true).
+    { clear -H0. induction H0; auto. destruct x. simpl in H0. simpl.
+      rewrite Nat.eqb_refl, H, IHForall. reflexivity. }
+    rewrite Hlres, H. reflexivity.
+  * rewrite Nat.eqb_refl, Nat.eqb_refl, H, H0, H1. reflexivity.
+  * induction H; auto. simpl. rewrite H, IHForall. reflexivity.
+  * destruct seg; simpl in *; rewrite H, H0, Nat.eqb_refl, BinSign_eqb_refl, BinType_eqb_refl, BinEnd_eqb_refl.
+    reflexivity.
+  (* Pattern *)
   * apply Lit_eqb_refl.
-  * apply Nat.eqb_refl.
-  * rewrite IHv1, IHv2. reflexivity.
-  * induction IHv; auto. rewrite H, IHIHv. reflexivity.
-  * induction IHv; auto. destruct x, H. simpl in *. rewrite H, H0, IHIHv. reflexivity.
-  * apply Nat.eqb_refl.
-  * destruct n. simpl. do 2 rewrite Nat.eqb_refl. reflexivity.
-  * rewrite IHv0, Nat.eqb_refl, Nat.eqb_refl. simpl.
-    clear -IHv. induction IHv; auto.
-    destruct x, p. simpl in H. rewrite IHIHv, H, Nat.eqb_refl, Nat.eqb_refl. reflexivity.
-  * now rewrite IHv, Nat.eqb_refl.
-  * induction IHv; auto. now rewrite H, IHIHv.
-  * now rewrite IHv, IHv0.
-  * induction IHv; auto. now rewrite H, IHIHv.
-  * induction IHv; auto. destruct x, H. simpl in *. now rewrite H, H0, IHIHv.
-  * rewrite IHv, IHv0. simpl.
-    clear -IHv1. induction IHv1; auto. now rewrite H, IHIHv1.
-  * rewrite String.eqb_refl. simpl. induction IHv; auto.
-    now rewrite H, IHIHv.
-  * rewrite IHv. simpl.
-    clear -IHv0. induction IHv0; auto. now rewrite H, IHIHv0.
-  * rewrite IHv, Nat.eqb_refl. simpl. induction IHv0; auto.
-    destruct x, p, H, H0. simpl in *. rewrite H, H0. simpl. rewrite IHIHv0.
-    clear -H1. induction H1; auto. rewrite H. simpl. rewrite IHForall. reflexivity.
-  * now rewrite IHv, IHv0, Nat.eqb_refl.
-  * now rewrite IHv, IHv0.
-  * rewrite IHv. induction IHv0; auto. destruct x. simpl in H.
-    rewrite Nat.eqb_refl. simpl in *. rewrite H. simpl. rewrite IHIHv0. reflexivity.
-  * now rewrite Nat.eqb_refl, Nat.eqb_refl, IHv, IHv0, IHv1.
-  * constructor; auto.
-    split. auto. split. auto.
-    induction l; constructor. apply Pat_eqb_refl. apply IHl.
+  * rewrite H, H0. reflexivity.
+  * induction H; auto. simpl. rewrite H, IHForall. reflexivity.
+  * induction H; auto. destruct x, H. simpl in *. rewrite H, H1, IHForall. reflexivity.
+  * induction H; auto. simpl. destruct H as [Hv Hs].
+    destruct x; simpl in *; rewrite Hv, Hs, Nat.eqb_refl, BinSign_eqb_refl, BinType_eqb_refl, BinEnd_eqb_refl, IHForall.
+    reflexivity.
 Qed.
 
-Lemma Val_eqb_strict_eq: forall v1 v2, Val_eqb_strict v1 v2 = true <-> v1 = v2.
-Proof.
-  intros. split.
-  * revert v2.
-    induction v1 using Val_ind2 with
-      (P  := fun e => forall e2, Exp_eqb_strict e e2 = true -> e = e2)
-      (PE := fun e => forall e2, Exp_eqb_strict e e2 = true -> e = e2)
-      (Q  := Forall (fun e => forall e2, Exp_eqb_strict e e2 = true -> e = e2))
-      (QV := Forall (fun v => forall v2, Val_eqb_strict v v2 = true -> v = v2))
-      (R  := Forall (PBoth (fun e => forall e2, Exp_eqb_strict e e2 = true -> e = e2)))
-      (RV := Forall (PBoth (fun v => forall v2, Val_eqb_strict v v2 = true -> v = v2)))
-      (VV := Forall (fun '(_, e) => forall e2, Exp_eqb_strict e e2 = true -> e = e2 ))
-      (W  := Forall (fun '(_, e, e') => (forall e2,  Exp_eqb_strict e  e2  = true -> e  = e2) /\
-                                        (forall e2', Exp_eqb_strict e' e2' = true -> e' = e2')))
-      (Z  := Forall (fun '(_, e) => forall e2, Exp_eqb_strict e e2 = true -> e = e2)); auto.
-    + intros. simpl in H. destruct e2; try discriminate.
-      apply IHv1 in H. subst. reflexivity.
-    + intros. simpl in H. destruct v2; try discriminate. reflexivity.
-    + intros. simpl in H. destruct v2; try discriminate. apply Lit_eqb_eq in H. subst. reflexivity.
-    + intros. simpl in H. destruct v2; try discriminate. apply Nat.eqb_eq in H. subst. reflexivity.
-    + intros. simpl in H. destruct v2; try discriminate.
-      apply andb_prop in H. destruct H.
-      apply IHv1_1 in H. apply IHv1_2 in H0. subst. reflexivity.
-    + intros. simpl in H. destruct v2; try discriminate.
-      revert H IHv1. revert l0. revert l. induction l; intros.
-      - destruct l0. reflexivity. discriminate.
-      - destruct l0. discriminate.
-        apply andb_prop in H. destruct H.
-        inv IHv1. apply H3 in H. subst a.
-        specialize (IHl l0 H0 H4). inv IHl. reflexivity.
-    + intros. simpl in H. destruct v2; try discriminate.
-      revert H IHv1. revert l0. revert l. induction l; intros.
-      - destruct l0. reflexivity. discriminate.
-      - destruct l0. destruct a. discriminate.
-        destruct a, p.
-        apply andb_prop in H. destruct H. apply andb_prop in H0. destruct H0.
-        inv IHv1. inv H4. simpl in H2, H3. apply H2 in H. apply H3 in H0. subst v v0.
-        specialize (IHl l0 H1 H5). inv IHl. reflexivity.
-    + intros. simpl in H. destruct v2; try discriminate. apply Nat.eqb_eq in H. subst. reflexivity.
-    + intros. simpl in H. destruct v2; try discriminate. unfold funid_eqb in H. destruct n, n0.
-      apply andb_prop in H. destruct H. apply Nat.eqb_eq in H, H0. subst. reflexivity.
-    + intros. simpl in H. destruct v2; try discriminate. apply andb_prop in H. destruct H.
-      apply andb_prop in H. destruct H. apply andb_prop in H. destruct H.
-      apply Nat.eqb_eq in H, H2. apply IHv0 in H1. subst id vl e.
-      revert H0 IHv1. revert ext0.
-      induction ext; intros.
-      - destruct ext0. reflexivity. discriminate.
-      - destruct a, p. destruct ext0. discriminate.
-        destruct p, p. apply andb_prop in H0. destruct H0.
-        apply andb_prop in H0. destruct H0. apply andb_prop in H1. destruct H1.
-        apply Nat.eqb_eq in H0, H1. inv IHv1. apply H5 in H. subst e.
-        specialize (IHext ext0 H2 H6). inv IHext. reflexivity.
-    + intros. simpl in H. destruct e2; try discriminate. destruct e0; try discriminate.
-      apply andb_prop in H. destruct H. apply Nat.eqb_eq in H.
-      apply IHv1 in H0. subst. reflexivity.
-    + intros. simpl in H. destruct e2; try discriminate. destruct e; try discriminate.
-      revert H IHv1. revert el0. revert el.
-      induction el; intros.
-      - destruct el0. reflexivity. discriminate.
-      - destruct el0. discriminate.
-        apply andb_prop in H. destruct H.
-        inv IHv1. apply H3 in H. subst a.
-        specialize (IHel el0 H0 H4). inv IHel. reflexivity.
-    + intros. simpl in H. destruct e2; try discriminate. destruct e; try discriminate.
-      apply andb_prop in H. destruct H.
-      apply IHv1 in H. apply IHv0 in H0. subst. reflexivity.
-    + intros. simpl in H. destruct e2; try discriminate. destruct e; try discriminate.
-      revert H IHv1. revert l0. revert l.
-      induction l; intros.
-      - destruct l0. reflexivity. discriminate.
-      - destruct l0. discriminate.
-        apply andb_prop in H. destruct H.
-        inv IHv1. apply H3 in H. subst a.
-        specialize (IHl l0 H0 H4). inv IHl. reflexivity.
-    + intros. simpl in H. destruct e2; try discriminate. destruct e; try discriminate.
-      revert H IHv1. revert l0.
-      induction l; intros.
-      - destruct l0. reflexivity. discriminate.
-      - destruct a. destruct l0. discriminate.
-        destruct p. apply andb_prop in H. destruct H. apply andb_prop in H0. destruct H0.
-        inv IHv1. inv H4. simpl in H2, H3. apply H2 in H. apply H3 in H0. subst e e0.
-        specialize (IHl l0 H1 H5). inv IHl. reflexivity.
-    + intros. simpl in H. destruct e2; try discriminate. destruct e; try discriminate.
-      apply andb_prop in H. destruct H. apply andb_prop in H. destruct H.
-      apply IHv1 in H1. apply IHv0 in H. subst f m.
-      revert H0 IHv2 IHv0 IHv1. revert l0.
-      induction l; intros.
-      - destruct l0. reflexivity. discriminate.
-      - destruct l0. discriminate.
-        apply andb_prop in H0. destruct H0. inv IHv2. apply H3 in H. subst a.
-        specialize (IHl l0 H0 H4 IHv0 IHv1). inv IHl. reflexivity.
-    + intros. simpl in H. destruct e2; try discriminate. destruct e; try discriminate.
-      apply andb_prop in H. destruct H.
-      apply String.eqb_eq in H. subst f.
-      revert H0 IHv1. revert l0.
-      induction l; intros.
-      - destruct l0. reflexivity. discriminate.
-      - destruct l0. discriminate.
-        apply andb_prop in H0. destruct H0. inv IHv1. apply H3 in H. subst a.
-        specialize (IHl l0 H0 H4). inv IHl. reflexivity.
-    + intros. simpl in H. destruct e2; try discriminate. destruct e0; try discriminate.
-      apply andb_prop in H. destruct H. apply IHv1 in H. subst e.
-      revert H0 IHv0. revert l0.
-      induction l; intros.
-      - destruct l0. reflexivity. discriminate.
-      - destruct l0. discriminate.
-        apply andb_prop in H0. destruct H0. inv IHv0. apply H3 in H. subst a.
-        specialize (IHl l0 H0 H4). inv IHl. reflexivity.
-    + intros. simpl in H. destruct e2; try discriminate. destruct e0; try discriminate.
-      apply andb_prop in H. destruct H. apply andb_prop in H. destruct H.
-      apply IHv1 in H. subst e.
-      revert H0 IHv0 H1. revert l0.
-      induction l; intros.
-      - destruct l0. reflexivity. discriminate.
-      - destruct l0. discriminate.
-        destruct a, p0, p, p.
-        apply andb_prop in H0. destruct H0. apply andb_prop in H0. destruct H0.
-        apply andb_prop in H2. destruct H2. inv IHv0. destruct H6.
-        apply H4 in H0. apply H5 in H2. subst e e1.
-        specialize (IHl l0 H3 H7 H1). inv IHl.
-        clear H3. clear -H.
-        revert H. revert l2.
-        induction l1; intros.
-        ** destruct l2. reflexivity. discriminate. 
-        ** destruct l2. discriminate.
-           apply andb_prop in H. destruct H. apply Pat_eqb_eq in H. subst a.
-           specialize (IHl1 l2 H0). inv IHl1. reflexivity.
-    + intros. simpl in H. destruct e0; try discriminate. destruct e; try discriminate.
-      apply andb_prop in H. destruct H. apply andb_prop in H. destruct H.
-      apply Nat.eqb_eq in H. apply IHv1 in H1. apply IHv0 in H0. subst. reflexivity.
-    + intros. simpl in H. destruct e0; try discriminate. destruct e; try discriminate.
-      apply andb_prop in H. destruct H.
-      apply IHv1 in H. apply IHv0 in H0. subst. reflexivity.
-    + intros. simpl in H. destruct e2; try discriminate. destruct e0; try discriminate.
-      apply andb_prop in H. destruct H. apply IHv1 in H0. subst e.
-      revert H IHv0. revert l0.
-      induction l; intros.
-      - destruct l0. reflexivity. discriminate.
-      - destruct a. destruct l0. discriminate.
-        destruct p. apply andb_prop in H. destruct H. apply andb_prop in H0. destruct H0.
-        apply Nat.eqb_eq in H. subst n. inv IHv0. apply H3 in H0. subst e.
-        specialize (IHl l0 H1 H4). inv IHl. reflexivity. 
-    + intros. simpl in H. destruct e0; try discriminate. destruct e; try discriminate.
-      apply andb_prop in H. destruct H. apply andb_prop in H. destruct H.
-      apply andb_prop in H. destruct H. apply andb_prop in H. destruct H.
-      apply Nat.eqb_eq in H, H3. apply IHv1 in H2. apply IHv0 in H1. apply IHv2 in H0.
-      subst. reflexivity.
-  * intro. rewrite H. apply Val_eqb_strict_refl.
-Qed.
+Corollary eqb_strict_refl : forall e, Exp_eqb_strict e e = true.
+Proof. now apply Private_eqb_strict_refl. Qed.
 
-Lemma Exp_eqb_strict_eq: forall e1 e2, Exp_eqb_strict e1 e2 = true <-> e1 = e2.
+Corollary eqb_strict_refl_nonval : forall e, NonVal_eqb_strict e e = true.
+Proof. now apply Private_eqb_strict_refl. Qed.
+
+Corollary eqb_strict_refl_val : forall v, Val_eqb_strict v v = true.
+Proof. now apply Private_eqb_strict_refl. Qed.
+
+Corollary eqb_strict_refl_pat : forall p, Pat_eqb_strict p p = true.
+Proof. now apply Private_eqb_strict_refl. Qed.
+
+Lemma Private_eqb_strict_eq_fwd :
+     (forall e1 e2, Exp_eqb_strict e1 e2 = true -> e1 = e2)
+  /\ (forall e1 e2, NonVal_eqb_strict e1 e2 = true -> e1 = e2)
+  /\ (forall v1 v2, Val_eqb_strict v1 v2 = true -> v1 = v2)
+  /\ (forall p1 p2, Pat_eqb_strict p1 p2 = true -> p1 = p2).
 Proof.
-  intros. split.
-  * revert e2.
-    induction e1 using Exp_ind2 with
-    (PV := fun _ => True)
-    (PE := fun e => forall e2, Exp_eqb_strict e e2 = true -> e = e2)
-    (Q  := Forall (fun e => forall e2, Exp_eqb_strict e e2 = true -> e = e2))
-    (QV := fun _ => True)
-    (R  := Forall (PBoth (fun e => forall e2, Exp_eqb_strict e e2 = true -> e = e2)))
-    (RV := fun _ => True)
-    (VV := fun _ => True)
-    (W  := Forall (fun '(_, e, e') => (forall e2,  Exp_eqb_strict e  e2  = true -> e  = e2) /\
-                                        (forall e2', Exp_eqb_strict e' e2' = true -> e' = e2')))
-    (Z  := Forall (fun '(_, e) => forall e2, Exp_eqb_strict e e2 = true -> e = e2)); auto.
-    + intros. simpl in H. destruct e2; try discriminate.
-      apply Val_eqb_strict_eq in H. subst. reflexivity.
-    + intros. simpl in H. destruct e2; try discriminate. destruct e; try discriminate.
-      apply andb_prop in H. destruct H.
-      apply Nat.eqb_eq in H. apply IHe1 in H0. subst. reflexivity.
-    + intros. simpl in H. destruct e2; try discriminate. destruct e; try discriminate.
-      revert H IHe1. revert el0.
-      induction el; intros.
+  apply Exp_ind with
+    (Q  := Forall (fun e1 => forall e2, Exp_eqb_strict e1 e2 = true -> e1 = e2))
+    (QV := Forall (fun v1 => forall v2, Val_eqb_strict v1 v2 = true -> v1 = v2))
+    (R  := Forall (PBoth (fun e1 => forall e2, Exp_eqb_strict e1 e2 = true -> e1 = e2)))
+    (RV := Forall (PBoth (fun v1 => forall v2, Val_eqb_strict v1 v2 = true -> v1 = v2)))
+    (VV := Forall (fun '(_,_,e1) => forall e2, Exp_eqb_strict e1 e2 = true -> e1 = e2))
+    (W  := Forall (fun '(lp,e1,e1') =>
+             Forall (fun p1 => forall p2, Pat_eqb_strict p1 p2 = true -> p1 = p2) lp
+             /\ (forall e2, Exp_eqb_strict e1 e2 = true -> e1 = e2)
+             /\ (forall e2, Exp_eqb_strict e1' e2 = true -> e1' = e2)))
+    (Z  := Forall (fun '(_,e1) => forall e2, Exp_eqb_strict e1 e2 = true -> e1 = e2))
+    (PQ := Forall (fun p1 => forall p2, Pat_eqb_strict p1 p2 = true -> p1 = p2))
+    (PR := Forall (PBoth (fun p1 => forall p2, Pat_eqb_strict p1 p2 = true -> p1 = p2)))
+    (PT := Forall (fun seg : Segment Pat Val =>
+             (forall p2, Pat_eqb_strict (Syntax.val seg) p2 = true -> Syntax.val seg = p2)
+             /\ (forall v2, Val_eqb_strict (Syntax.size seg) v2 = true -> Syntax.size seg = v2)))
+  ; simpl; auto; intros.
+  (* Exp/NonVal wrappers *)
+  * destruct e2; try discriminate. apply H in H0. subst. reflexivity.
+  * destruct e2; try discriminate. apply H in H0. subst. reflexivity.
+  (* Val *)
+  * destruct v2; try discriminate. reflexivity.
+  * destruct v2; try discriminate. apply Lit_eqb_eq in H. subst. reflexivity.
+  * destruct v2; try discriminate. apply Nat.eqb_eq in H. subst. reflexivity.
+  * destruct v2; try discriminate. apply andb_prop in H1. destruct H1.
+    apply H in H1. apply H0 in H2. subst. reflexivity.
+  * destruct v2; try discriminate.
+    assert (l = l0).
+    { revert H0. revert l0. induction H; intros.
+      - destruct l0; try discriminate. reflexivity.
+      - destruct l0; try discriminate. simpl in H1. apply andb_prop in H1. destruct H1.
+        apply H in H1. f_equal; auto. }
+    subst. reflexivity.
+  * destruct v2; try discriminate.
+    assert (l = l0).
+    { revert H0. revert l0. induction H; intros.
+      - destruct l0; try discriminate. reflexivity.
+      - destruct l0; try discriminate. destruct x, p.
+        destruct H as [Hx Hy]. simpl in H1. apply andb_prop in H1. destruct H1.
+        apply andb_prop in H. destruct H as [Ha Hb]. simpl in Hx, Hy.
+        apply Hx in Ha. apply Hy in Hb. apply IHForall in H1.
+        subst. reflexivity. }
+    subst. reflexivity.
+  * destruct v2; try discriminate. apply Nat.eqb_eq in H. subst. reflexivity.
+  * destruct v2; try discriminate. unfold funid_eqb in H. destruct n, n0.
+    apply andb_prop in H. destruct H. apply Nat.eqb_eq in H, H0. subst. reflexivity.
+  * destruct v2; try discriminate.
+    apply andb_prop in H1. destruct H1. apply andb_prop in H1. destruct H1.
+    apply andb_prop in H1. destruct H1. apply Nat.eqb_eq in H1, H4.
+    apply H0 in H3. subst id vl e.
+    assert (ext = ext0).
+    { revert H2. revert ext0. induction H; intros.
+      - destruct ext0; try discriminate. reflexivity.
+      - destruct ext0; try discriminate. destruct x, p, p0, p.
+        simpl in H2. apply andb_prop in H2. destruct H2. apply andb_prop in H2. destruct H2.
+        apply andb_prop in H2. destruct H2. apply Nat.eqb_eq in H2, H5.
+        apply H in H4. apply IHForall in H3.
+        subst. reflexivity. }
+    subst. reflexivity.
+  * destruct v2; try discriminate. destruct (bvn_eq_dec b bits); [subst; reflexivity | discriminate].
+  (* NonVal *)
+  * destruct e2; try discriminate. apply andb_prop in H0. destruct H0.
+    apply Nat.eqb_eq in H0. apply H in H1. subst. reflexivity.
+  * destruct e2; try discriminate.
+    assert (el = el0).
+    { revert H0. revert el0. induction H; intros.
       - destruct el0; try discriminate. reflexivity.
-      - destruct el0. discriminate.
-        apply andb_prop in H. destruct H.
-        inv IHe1. apply H3 in H. subst a.
-        specialize (IHel el0 H0 H4). inv IHel. reflexivity.
-    + intros. simpl in H. destruct e2; try discriminate. destruct e; try discriminate.
-      apply andb_prop in H. destruct H.
-      apply IHe1_1 in H. apply IHe1_2 in H0. subst. reflexivity.
-    + intros. simpl in H. destruct e2; try discriminate. destruct e; try discriminate.
-      revert H IHe1. revert l0.
-      induction l; intros.
+      - destruct el0; try discriminate. simpl in H1. apply andb_prop in H1. destruct H1.
+        apply H in H1. f_equal; auto. }
+    subst. reflexivity.
+  * destruct e2; try discriminate. apply andb_prop in H1. destruct H1.
+    apply H in H1. apply H0 in H2. subst. reflexivity.
+  * destruct e2; try discriminate.
+    assert (l = l0).
+    { revert H0. revert l0. induction H; intros.
       - destruct l0; try discriminate. reflexivity.
-      - destruct l0. discriminate.
-        apply andb_prop in H. destruct H.
-        inv IHe1. apply H3 in H. subst a.
-        specialize (IHl l0 H0 H4). inv IHl. reflexivity.
-    + intros. simpl in H. destruct e2; try discriminate. destruct e; try discriminate.
-      revert H IHe1. revert l0.
-      induction l; intros.
+      - destruct l0; try discriminate. simpl in H1. apply andb_prop in H1. destruct H1.
+        apply H in H1. f_equal; auto. }
+    subst. reflexivity.
+  * destruct e2; try discriminate.
+    assert (l = l0).
+    { revert H0. revert l0. induction H; intros.
       - destruct l0; try discriminate. reflexivity.
-      - destruct a. destruct l0. discriminate.
-        destruct p. apply andb_prop in H. destruct H. apply andb_prop in H0. destruct H0.
-        inv IHe1. inv H4. apply H2 in H. apply H3 in H0. subst e1 e2.
-        specialize (IHl l0 H1 H5). inv IHl. reflexivity.
-    + intros. simpl in H. destruct e2; try discriminate. destruct e; try discriminate.
-      apply andb_prop in H. destruct H. apply andb_prop in H. destruct H.
-      apply IHe1_2 in H. apply IHe1_1 in H1. subst f m.
-      revert H0 IHe1_3. revert l0.
-      induction l; intros.
+      - destruct l0; try discriminate. destruct x, p.
+        destruct H as [Hx Hy]. simpl in Hx, Hy. simpl in H1.
+        apply andb_prop in H1. destruct H1. apply andb_prop in H. destruct H as [Ha Hb].
+        apply Hx in Ha. apply Hy in Hb. apply IHForall in H1.
+        subst. reflexivity. }
+    subst. reflexivity.
+  * destruct e2; try discriminate.
+    apply andb_prop in H2. destruct H2. apply andb_prop in H2. destruct H2.
+    apply H0 in H2. apply H in H4. subst f m.
+    assert (l = l0).
+    { clear -H1 H3. revert H3. revert l0. induction H1; intros.
       - destruct l0; try discriminate. reflexivity.
-      - destruct l0. discriminate.
-        apply andb_prop in H0. destruct H0.
-        inv IHe1_3. apply H3 in H. subst a.
-        specialize (IHl l0 H0 H4). inv IHl. reflexivity.
-    + intros. simpl in H. destruct e2; try discriminate. destruct e; try discriminate.
-      apply andb_prop in H. destruct H.
-      apply String.eqb_eq in H. subst f.
-      revert H0 IHe1. revert l0.
-      induction l; intros.
+      - destruct l0; try discriminate. simpl in H3. apply andb_prop in H3. destruct H3.
+        apply H in H0. f_equal; auto. }
+    subst. reflexivity.
+  * destruct e2; try discriminate. apply andb_prop in H0. destruct H0.
+    apply String.eqb_eq in H0. subst f0.
+    assert (l = l0).
+    { clear -H H1. revert H1. revert l0. induction H; intros.
       - destruct l0; try discriminate. reflexivity.
-      - destruct l0. discriminate.
-        apply andb_prop in H0. destruct H0.
-        inv IHe1. apply H3 in H. subst a.
-        specialize (IHl l0 H0 H4). inv IHl. reflexivity.
-    + intros. simpl in H. destruct e2; try discriminate. destruct e; try discriminate.
-      apply andb_prop in H. destruct H.
-      apply IHe1 in H. subst e1.
-      revert H0 IHe0. revert l0.
-      induction l; intros.
+      - destruct l0; try discriminate. simpl in H1. apply andb_prop in H1. destruct H1.
+        apply H in H1. f_equal; auto. }
+    subst. reflexivity.
+  * destruct e2; try discriminate. apply andb_prop in H1. destruct H1.
+    apply H in H1. subst e.
+    assert (l = l0).
+    { clear -H0 H2. revert H2. revert l0. induction H0; intros.
       - destruct l0; try discriminate. reflexivity.
-      - destruct l0. discriminate.
-        apply andb_prop in H0. destruct H0.
-        inv IHe0. apply H3 in H. subst a.
-        specialize (IHl l0 H0 H4). inv IHl. reflexivity.
-    + intros. simpl in H. destruct e2; try discriminate. destruct e; try discriminate.
-      apply andb_prop in H. destruct H. apply andb_prop in H. destruct H. clear H1.
-      apply IHe1 in H. subst e.
-      revert H0 IHe0. revert l0.
-      induction l; intros.
+      - destruct l0; try discriminate. simpl in H2. apply andb_prop in H2. destruct H2.
+        apply H in H1. apply IHForall in H2.
+        subst. reflexivity. }
+    subst. reflexivity.
+  * destruct e2; try discriminate.
+    apply andb_prop in H1. destruct H1. apply andb_prop in H1. destruct H1.
+    apply H in H1. subst e. clear H3.
+    assert (l = l0).
+    { clear -H0 H2. revert H2. revert l0. induction H0; intros.
       - destruct l0; try discriminate. reflexivity.
-      - destruct a, p. destruct l0. discriminate.
-        destruct p, p.
-        apply andb_prop in H0. destruct H0. apply andb_prop in H0. destruct H0.
-        apply andb_prop in H1. destruct H1.
-        inv IHe0. destruct H5.
-        apply H3 in H0. apply H4 in H1. subst e0 e.
-        specialize (IHl l0 H2 H6). inv IHl.
-        clear -H. revert H. revert l2.
-        induction l1; intros.
-        ** destruct l2; try discriminate. reflexivity. 
-        ** destruct l2. discriminate.
-           apply andb_prop in H. destruct H.
-           apply Pat_eqb_eq in H. subst a.
-           specialize (IHl1 l2 H0). inv IHl1. reflexivity.
-    + intros. simpl in H. destruct e2;try discriminate. destruct e; try discriminate.
-      apply andb_prop in H. destruct H. apply andb_prop in H. destruct H.
-      apply IHe1_1 in H1. apply IHe1_2 in H0. apply Nat.eqb_eq in H. subst. reflexivity.
-    + intros. simpl in H. destruct e2; try discriminate. destruct e; try discriminate.
-      apply andb_prop in H. destruct H. apply IHe1_1 in H. apply IHe1_2 in H0.
-      subst. reflexivity.
-    + intros. simpl in H. destruct e2; try discriminate. destruct e; try discriminate.
-      revert H IHe0. revert l0.
-      induction l; intros.
-      - destruct l0; try discriminate.
-        simpl in H. apply IHe1 in H. subst. reflexivity.
-      - destruct a. destruct l0. discriminate.
-        destruct p. apply andb_prop in H. destruct H. apply andb_prop in H. destruct H.
-        apply andb_prop in H1. destruct H1.
-        apply IHe1 in H0. apply Nat.eqb_eq in H.
-        inv IHe0. apply H5 in H1. subst.
-        setoid_rewrite Exp_eqb_strict_refl in IHl.
-        setoid_rewrite andb_comm in IHl. simpl in IHl.
-        specialize (IHl l0 H2 H6). inv IHl. reflexivity.
-    + intros. simpl in H. destruct e2; try discriminate. destruct e; try discriminate.
-      apply andb_prop in H. destruct H. apply andb_prop in H. destruct H.
-      apply andb_prop in H. destruct H. apply andb_prop in H. destruct H.
-      apply IHe1_1 in H2. apply IHe1_2 in H1. apply IHe1_3 in H0.
-      apply Nat.eqb_eq in H, H3. subst. reflexivity.
-  * intro. rewrite H. apply Exp_eqb_strict_refl.
+      - destruct l0; try discriminate. destruct x as [[lp e1] e1']. destruct p as [[lp' ea] eb].
+        destruct H as [Hlp [He1 He1']]. simpl in H2. apply andb_prop in H2. destruct H2.
+        apply andb_prop in H. destruct H. apply andb_prop in H. destruct H.
+        apply He1 in H3. apply He1' in H2. apply IHForall in H1.
+        assert (lp = lp').
+        { clear -Hlp H. revert H. revert lp'. induction Hlp; intros.
+          - destruct lp'; try discriminate. reflexivity.
+          - destruct lp'; try discriminate. simpl in H0. apply andb_prop in H0. destruct H0.
+            apply H in H0. f_equal; auto. }
+        subst. reflexivity. }
+    subst. reflexivity.
+  * destruct e0; try discriminate.
+    apply andb_prop in H1. destruct H1. apply andb_prop in H1. destruct H1.
+    apply Nat.eqb_eq in H1. apply H in H3. apply H0 in H2. subst. reflexivity.
+  * destruct e0; try discriminate. apply andb_prop in H1. destruct H1.
+    apply H in H1. apply H0 in H2. subst. reflexivity.
+  * destruct e2; try discriminate. apply andb_prop in H1. destruct H1.
+    apply H in H2. subst e.
+    assert (l = l0).
+    { clear -H0 H1. revert H1. revert l0. induction H0; intros.
+      - destruct l0; try discriminate. reflexivity.
+      - destruct l0; try discriminate. destruct x, p.
+        simpl in H1. apply andb_prop in H1. destruct H1. apply andb_prop in H1. destruct H1.
+        apply Nat.eqb_eq in H1. apply H in H3. apply IHForall in H2.
+        subst. reflexivity. }
+    subst. reflexivity.
+  * destruct e0; try discriminate.
+    apply andb_prop in H2. destruct H2. apply andb_prop in H2. destruct H2.
+    apply andb_prop in H2. destruct H2. apply andb_prop in H2. destruct H2.
+    apply Nat.eqb_eq in H2, H6. apply H in H5. apply H0 in H4. apply H1 in H3.
+    subst. reflexivity.
+  * destruct e2; try discriminate.
+    assert (l = l0).
+    { clear -H H0. revert H0. revert l0. induction H; intros.
+      - destruct l0; try discriminate. reflexivity.
+      - destruct l0; try discriminate. simpl in H1. apply andb_prop in H1. destruct H1.
+        apply H in H1. f_equal; auto. }
+    subst. reflexivity.
+  * destruct e2; try discriminate. destruct seg, seg0. simpl in *.
+    repeat (apply andb_prop in H1; destruct H1).
+    apply H in H1. apply H0 in H6. apply Nat.eqb_eq in H5.
+    apply BinType_eqb_eq in H4. apply BinSign_eqb_eq in H3. apply BinEnd_eqb_eq in H2.
+    subst. reflexivity.
+  (* Pattern *)
+  * destruct p2; try discriminate. reflexivity.
+  * destruct p2; try discriminate. apply Lit_eqb_eq in H. subst. reflexivity.
+  * destruct p2; try discriminate. reflexivity.
+  * destruct p2; try discriminate. apply andb_prop in H1. destruct H1.
+    apply H in H1. apply H0 in H2. subst. reflexivity.
+  * destruct p2; try discriminate.
+    assert (l = l0).
+    { clear -H H0. revert H0. revert l0. induction H; intros.
+      - destruct l0; try discriminate. reflexivity.
+      - destruct l0; try discriminate. simpl in H1. apply andb_prop in H1. destruct H1.
+        apply H in H1. f_equal; auto. }
+    subst. reflexivity.
+  * destruct p2; try discriminate.
+    assert (l = l0).
+    { clear -H H0. revert H0. revert l0. induction H; intros.
+      - destruct l0; try discriminate. reflexivity.
+      - destruct l0; try discriminate. destruct x, p.
+        destruct H as [Hx Hy]. simpl in Hx, Hy. simpl in H1.
+        apply andb_prop in H1. destruct H1. apply andb_prop in H. destruct H as [Ha Hb].
+        apply Hx in Ha. apply Hy in Hb. apply IHForall in H1.
+        subst. reflexivity. }
+    subst. reflexivity.
+  * destruct p2; try discriminate.
+    assert (l = segments).
+    { clear -H H0. revert H0. revert segments. induction H; intros.
+      - destruct segments; try discriminate. reflexivity.
+      - destruct segments; try discriminate. destruct x, H as [Hv Hs]. destruct s. simpl in *.
+        repeat (apply andb_prop in H0; destruct H0).
+        repeat (apply andb_prop in H1; destruct H1).
+        repeat (apply andb_prop in H; destruct H).
+        apply Hv in H. apply Hs in H6. apply Nat.eqb_eq in H5.
+        apply BinType_eqb_eq in H4. apply BinSign_eqb_eq in H3. apply BinEnd_eqb_eq in H2.
+        apply IHForall in H1.
+        subst. reflexivity. }
+    subst. reflexivity.
 Qed.
+
+Theorem Private_eqb_strict_eq :
+     (forall e1 e2, Exp_eqb_strict e1 e2 = true <-> e1 = e2)
+  /\ (forall e1 e2, NonVal_eqb_strict e1 e2 = true <-> e1 = e2)
+  /\ (forall v1 v2, Val_eqb_strict v1 v2 = true <-> v1 = v2)
+  /\ (forall p1 p2, Pat_eqb_strict p1 p2 = true <-> p1 = p2).
+Proof.
+  destruct Private_eqb_strict_eq_fwd as [F1 [F2 [F3 F4]]].
+  destruct Private_eqb_strict_refl as [R1 [R2 [R3 R4]]].
+  split; [| split; [| split]].
+  - intros e1 e2. split. apply F1. intros; subst; apply R1.
+  - intros e1 e2. split. apply F2. intros; subst; apply R2.
+  - intros v1 v2. split. apply F3. intros; subst; apply R3.
+  - intros p1 p2. split. apply F4. intros; subst; apply R4.
+Qed.
+
+Corollary eqb_strict_eq : forall e1 e2, Exp_eqb_strict e1 e2 = true <-> e1 = e2.
+Proof. apply Private_eqb_strict_eq. Qed.
+
+Corollary eqb_strict_eq_nonval : forall e1 e2, NonVal_eqb_strict e1 e2 = true <-> e1 = e2.
+Proof. apply Private_eqb_strict_eq. Qed.
+
+Corollary eqb_strict_eq_val : forall v1 v2, Val_eqb_strict v1 v2 = true <-> v1 = v2.
+Proof. apply Private_eqb_strict_eq. Qed.
+
+Corollary eqb_strict_eq_pat : forall p1 p2, Pat_eqb_strict p1 p2 = true <-> p1 = p2.
+Proof. apply Private_eqb_strict_eq. Qed.
 
 Lemma Val_eqb_strict_lit_eqb: forall v l, Val_eqb_strict v (VLit l) = Val_eqb v (VLit l).
 Proof.
