src/FrameStack/Frames.v
@@ -86,13 +86,13 @@ Inductive FCLOSED : Frame -> Prop :=
 | fclosed_callmod f l : EXPCLOSED f -> Forall (fun e => EXPCLOSED e) l -> FCLOSED (FCallMod f l)
 | fclosed_callfun m l : VALCLOSED m -> Forall (fun e => EXPCLOSED e) l -> FCLOSED (FCallFun m l)
 | fclosed_case1 l : 
-  Forall (fun '(pl, g, b) => EXP PatListScope pl ⊢ g /\ EXP PatListScope pl ⊢ b) l
+  Forall (fun '(pl, g, b) => Forall (PatScoped 0) pl /\ EXP PatListVars pl ⊢ g /\ EXP PatListVars pl ⊢ b) l
 ->
   FCLOSED (FCase1 l)
 | fclosed_case2 vl (* pl *) e rest :
   Forall (fun v => VALCLOSED v) vl ->
   EXPCLOSED e ->
-  Forall (fun '(pl, g, b) => EXP PatListScope pl ⊢ g /\ EXP PatListScope pl ⊢ b) rest
+  Forall (fun '(pl, g, b) => Forall (PatScoped 0) pl /\ EXP PatListVars pl ⊢ g /\ EXP PatListVars pl ⊢ b) rest
 ->
   FCLOSED (FCase2 vl (* pl *) e rest)
 | fclosed_let vars e : EXP vars ⊢ e -> FCLOSED (FLet vars e)
@@ -106,42 +106,57 @@ Inductive FCLOSED : Frame -> Prop :=
 Proposition clause_scope l :
   (forall i : nat,
   i < Datatypes.length l ->
-  EXP PatListScope (nth i (map (fst ∘ fst) l) [])
+  EXP PatListVars (nth i (map (fst ∘ fst) l) [])
   ⊢ nth i (map (snd ∘ fst) l) (˝ VNil)) ->
   (forall i : nat,
         i < Datatypes.length l ->
-        EXP PatListScope (nth i (map (fst ∘ fst) l) [])
+        EXP PatListVars (nth i (map (fst ∘ fst) l) [])
         ⊢ nth i (map snd l) (˝ VNil)) ->
-   Forall (fun '(pl, g, b) => EXP PatListScope pl ⊢ g /\ EXP PatListScope pl ⊢ b) l.
+  (forall i, i < length l -> forall j, j < length (nth i (map (fst ∘ fst) l) []) ->
+    PAT 0 ⊢ nth j (nth i (map (fst ∘ fst) l) []) PNil) ->
+   Forall (fun '(pl, g, b) => Forall (PatScoped 0) pl /\ EXP PatListVars pl ⊢ g /\ EXP PatListVars pl ⊢ b) l.
 Proof.
   induction l; intros; auto.
   constructor.
-  * destruct a, p. split.
+  * destruct a, p. split. 2: split.
+    - specialize (H1 0 ltac:(slia)).
+      rewrite indexed_to_forall. intros.
+      setoid_rewrite map_nth with (d := ([], ˝VNil, ˝VNil)) in H1. cbn in H1.
+      specialize (H1 i ltac:(lia)).
+      exact H1.
     - apply (H 0). slia.
     - apply (H0 0). slia.
-  * apply IHl; intros; (apply (H (S i)) + apply (H0 (S i))); slia.
+  * apply IHl; intros; (apply (H (S i)) + apply (H0 (S i)) + apply (H1 (S i))); slia.
 Qed.
 
 Proposition clause_scope_rev l :
-  Forall (fun '(pl, g, b) => EXP PatListScope pl ⊢ g /\ EXP PatListScope pl ⊢ b) l
+  Forall (fun '(pl, g, b) => Forall (PatScoped 0) pl /\ EXP PatListVars pl ⊢ g /\ EXP PatListVars pl ⊢ b) l
   ->
   (forall i : nat,
   i < Datatypes.length l ->
-  EXP PatListScope (nth i (map (fst ∘ fst) l) [])
+  EXP PatListVars (nth i (map (fst ∘ fst) l) [])
   ⊢ nth i (map (snd ∘ fst) l) (˝ VNil)) /\
   (forall i : nat,
         i < Datatypes.length l ->
-        EXP PatListScope (nth i (map (fst ∘ fst) l) [])
-        ⊢ nth i (map snd l) (˝ VNil))
+        EXP PatListVars (nth i (map (fst ∘ fst) l) [])
+        ⊢ nth i (map snd l) (˝ VNil)) /\
+  (forall i, i < length l -> forall j, j < length (nth i (map (fst ∘ fst) l) []) ->
+    PAT 0 ⊢ nth j (nth i (map (fst ∘ fst) l) []) PNil)
    .
 Proof.
-  intros. induction H; simpl; split; intros; try lia; destruct_foralls.
+  intros. induction H; simpl; repeat split; intros; try lia; destruct_foralls.
   * destruct i.
     - now destruct x, p, H.
     - apply IHForall. lia.
   * destruct i.
     - now destruct x, p, H0.
     - apply IHForall. lia.
+  * destruct i.
+    - destruct x, p; simpl in *.
+      destruct H as [H _].
+      rewrite indexed_to_forall in H.
+      by apply H.
+    - apply IHForall; lia.
 Qed.
 
 Definition to_Exp (ident : FrameIdent) (l : list Exp) : Exp :=
@@ -230,6 +245,7 @@ Ltac destruct_scopes :=
 Ltac scope_solver_step :=
   match goal with 
   | |- EXP _ ⊢ _ => constructor; simpl; auto
+  | |- PAT _ ⊢ _ => constructor; simpl; auto
   | |- VAL _ ⊢ _ => constructor; simpl; auto
   | |- RED _ ⊢ _ => constructor; simpl; auto
   | |- NVAL _ ⊢ _ => constructor; simpl; auto
@@ -245,6 +261,7 @@ Ltac scope_solver_step :=
   | [H : ?i < _ |- _] => inv H; simpl in *; auto; try lia
   | [H : ?i <= _ |- _] => inv H; simpl in *; auto; try lia
   | [H : EXP ?n1 ⊢ ?e |- EXP ?n2 ⊢ ?e] => try now (eapply (loosen_scope_exp n2 n1 ltac:(lia)) in H)
+  | [H : PAT ?n1 ⊢ ?e |- PAT ?n2 ⊢ ?e] => try now (eapply (loosen_scope_pat n2 n1 ltac:(lia)) in H)
   | [H : VAL ?n1 ⊢ ?e |- VAL ?n2 ⊢ ?e] => try now (eapply (loosen_scope_val n2 n1 ltac:(lia)) in H)
   | [H : NVAL ?n1 ⊢ ?e |- NVAL ?n2 ⊢ ?e] => try now (eapply (loosen_scope_nonval n2 n1 ltac:(lia)) in H)
   end.
