src/FrameStack/LabeledTermination.v
@@ -180,14 +180,14 @@ Inductive terminates_in_k : FrameStack -> Redex -> SideEffectList -> nat -> Prop
    e1 the guard needs to be evaluated. vs' (the result of the pattern
    matching is stored in the frame) *)
 | step_case_match lp e1 e2 l vs vs' xs ls k:
-  match_pattern_list lp vs = Some vs' ->
+  match_pattern_list lp vs = Matches vs' ->
   ⟨ (FCase2 vs e2.[list_subst vs' idsubst] l)::xs, RExp (e1.[list_subst vs' idsubst]) ⟩ ls – k ↓
 ->
   ⟨ (FCase1 ((lp,e1,e2)::l))::xs, RValSeq vs ⟩ ls – S k ↓
 (* reduction started or it is already ongoing, the first pattern doesn't 
    match, so we check the next pattern *)
 | step_case_not_match lp e1 e2 l vs xs ls k:
-  match_pattern_list lp vs = None ->
+  match_pattern_list lp vs = NotMatches ->
   ⟨ (FCase1 l)::xs, RValSeq vs ⟩ ls – k ↓ 
 ->
   ⟨ (FCase1 ((lp,e1,e2)::l))::xs, RValSeq vs ⟩ ls – S k ↓
